Roolean/QfBv/AbstractDomain.lean
@@ -32,11 +32,20 @@ public class AbstractDomain (α : Nat → Type) [Domain α] where
 public theorem AbstractDomain.choice_within {w} {α} [Domain α] [AbstractDomain α] (a: α w)
   : γ (a) (AbstractDomain.choice a).val = true := by simp[(AbstractDomain.choice a).property]
 
+public theorem AbstractDomain.implies_sound {α} [Domain α] [AbstractDomain α]
+  (aAnte aConse: α 1) (cAnte cConse: Bitvector 1)
+  : γ aAnte cAnte → γ aConse cConse → γ (Domain.implies aAnte aConse) (Domain.implies cAnte cConse) := by
+  intro hAnte hConse
+  simp(zeta:=false)[Domain.implies]
+  extract_lets aNotAnte cNotAnte
+  let hNotAnte := AbstractDomain.uniOp_sound aAnte cAnte UniOp.Not hAnte
+  exact AbstractDomain.biNormal_sound aNotAnte aConse BiNormalOp.BitOr cNotAnte cConse hNotAnte hConse
+
 public theorem AbstractDomain.concat_sound {α} [Domain α] [AbstractDomain α]
   (wl wr: Nat) (al: α wl) (ar: α wr) (cl: Bitvector wl) (cr: Bitvector wr)
   : γ al cl → γ ar cr → γ (Domain.concat wl wr al ar) (Domain.concat wl wr cl cr) := by
   intro hL hR
-  simp(zeta:= false)[Domain.concat]
+  simp(zeta:=false)[Domain.concat]
   extract_lets width aLeft aRight shiftValue aShift aShifted
     cLeft cRight cShift cShifted
   let hLeft := AbstractDomain.extOp_sound al cl (wl+wr) ExtOp.Uext hL
@@ -49,7 +58,7 @@ public theorem AbstractDomain.extract_sound {w} {α} [Domain α] [AbstractDomain
   (a: α w) (c: Bitvector w) (lsb: Fin w) (m: Nat)
   : γ a c → γ (Domain.extract a lsb m) (Domain.extract c lsb m) := by
   intro h
-  simp(zeta:= false)[Domain.extract]
+  simp(zeta:=false)[Domain.extract]
   extract_lets shiftValue aShift aShifted cShift cShifted
   let hShiftValue := AbstractDomain.ofBitvector_sound (α:=α) shiftValue
   let hShifted := AbstractDomain.biNormal_sound a aShift BiNormalOp.Lshr c cShift h hShiftValue
